

1 Bosonic string on a torus

1.1

The torus partition function on a circle S^1 of Radius R is given by

$$Z^{25} = \text{Tr} q^{L_0 - \frac{1}{24}} \bar{q}^{\bar{L}_0 - \frac{1}{24}} \quad (1.1)$$

L_0 and \bar{L}_0 are zero mode virasoro generators

$$L_0 = \frac{\alpha' p_L^2}{4} + \sum_{n=1}^{\infty} \hat{\alpha}_{-n} \hat{\alpha}_n \quad (1.2)$$

$$\bar{L}_0 = \frac{\alpha' p_R^2}{4} + \sum_{n=1}^{\infty} \hat{\bar{\alpha}}_{-n} \hat{\bar{\alpha}}_n \quad (1.3)$$

with right and left momentum

$$p_L = \frac{n}{R} + \frac{wR}{\alpha'} \quad (1.4)$$

$$p_R = \frac{n}{R} - \frac{wR}{\alpha'} \quad (1.5)$$

Then we can express Z^{25} in terms of Dedekind η function

$$\begin{aligned} Z^{25} &= (q\bar{q})^{-\frac{1}{24}} \text{Tr} q^{\frac{\alpha' p_L^2}{4} + \sum_{n=1}^{+\infty} \hat{\alpha}_{-n} \hat{\alpha}_n} \bar{q}^{\frac{\alpha' p_R^2}{4} + \sum_{n=1}^{+\infty} \hat{\bar{\alpha}}_{-n} \hat{\bar{\alpha}}_n} \\ &= (q\bar{q})^{-\frac{1}{24}} \sum_{n,w=-\infty}^{+\infty} q^{\frac{\alpha' p_L^2}{4}} \bar{q}^{\frac{\alpha' p_R^2}{4}} \sum_{N_n, \tilde{N}_n=0}^{+\infty} q^{nN_n} \bar{q}^{n\tilde{N}_n} \\ &= (q\bar{q})^{-\frac{1}{24}} \sum_{n,w=-\infty}^{+\infty} q^{\frac{\alpha' p_L^2}{4}} \bar{q}^{\frac{\alpha' p_R^2}{4}} \prod_{n=1}^{+\infty} |1 - q^n|^{-2} \\ &= |\eta(q)|^{-2} \sum_{n,w=-\infty}^{+\infty} q^{\frac{\alpha' p_L^2}{4}} \bar{q}^{\frac{\alpha' p_R^2}{4}} \end{aligned} \quad (1.6)$$

The partition function for the non-compact space $\mathbb{R}^{1,24}$

$$Z^{1,24} = \text{const} \times |\eta(q)|^{-46} \quad (1.7)$$

The matter part contributes $|\eta(q)|^{-50}$ (25 dimension), and the ghost part contribute $|\eta(q)|^4$ as usual.

To recover each mass formula term. We need expand the whole partion function.

$$\begin{aligned}
Z^{1,24} Z^{25} &= |\eta(q)|^{-46} |\eta(q)|^{-2} \sum_{n,w=-\infty}^{+\infty} q^{\frac{\alpha' p_L^2}{4}} \bar{q}^{\frac{\alpha' p_R^2}{4}} \\
&= [(q\bar{q})^{-\frac{1}{24}} \prod_{n=1}^{+\infty} (1-q^n)^{-1} (1-\bar{q}^n)^{-1}]^{24} \sum_{n,w=-\infty}^{+\infty} q^{\frac{\alpha' p_L^2}{4}} \bar{q}^{\frac{\alpha' p_R^2}{4}} \\
&= [(q\bar{q})^{-\frac{1}{24}} \prod_{n=1}^{+\infty} \sum_{N_n=0}^{+\infty} q^{nN_n} \sum_{\tilde{N}_n=0}^{+\infty} \bar{q}^{n\tilde{N}_n}]^{24} \sum_{n,w=-\infty}^{+\infty} q^{\frac{\alpha' p_L^2}{4}} \bar{q}^{\frac{\alpha' p_R^2}{4}} \\
&= \sum_{N_n=0}^{+\infty} \sum_{\tilde{N}_n=0}^{+\infty} \sum_{n,w=-\infty}^{+\infty} q^{\frac{\alpha' p_L^2}{4} - 1 + \sum_{n=1}^{\infty} 24nN_n} \bar{q}^{\frac{\alpha' p_R^2}{4} - 1 + \sum_{n=1}^{\infty} 24n\tilde{N}_n} \quad (1.8)
\end{aligned}$$

The number of state: Pochinski (1.3.37)

$$N = \sum_{D=1}^{D-1} \sum_{n=1}^{+\infty} n N_{im} \quad (1.9)$$

Where D is dimension. Rewrite the partition function

$$Z^{1,24} Z^{25} = \sum_{N_n=0}^{+\infty} \sum_{\tilde{N}_n=0}^{+\infty} \sum_{n,w=-\infty}^{+\infty} q^{\frac{\alpha' p_L^2}{4} - 1 + N} \bar{q}^{\frac{\alpha' p_R^2}{4} - 1 + \tilde{N}} \quad (1.10)$$

For each term, which means for each fixed N_n, \tilde{N}_n, n and w , it should be real which gives the level matching conditon

$$\begin{aligned}
0 &= \frac{\alpha' p_L^2}{4} + N - \frac{\alpha' p_R^2}{4} - \tilde{N} \\
&= \frac{\alpha'}{4} \times \frac{4nw}{\alpha'} + N - \tilde{N} \\
&= nw + N - \tilde{N} \quad (1.11)
\end{aligned}$$

Which is the desired level matching condition. The partition function now writes

$$\begin{aligned}
Z^{1,24} Z^{25} &= \sum_{N_n=0}^{+\infty} \sum_{\tilde{N}_n=0}^{+\infty} \sum_{n,w=-\infty}^{+\infty} |q|^{\frac{\alpha' p_L^2}{4} - 1 + N + \frac{\alpha' p_R^2}{4} - 1 + \tilde{N}} \\
&= \sum_{N_n=0}^{+\infty} \sum_{\tilde{N}_n=0}^{+\infty} \sum_{n,w=-\infty}^{+\infty} |q|^{\frac{\alpha'}{2} \left[\frac{n^2}{R^2} + \frac{\omega^2 R^2}{\alpha'^2} + \frac{2}{\alpha'} (N + \tilde{N} - 2) \right]} \quad (1.12)
\end{aligned}$$

So each term means the right hand sides of the mass formula $M^2 = \frac{n^2}{R^2} + \frac{\omega^2 R^2}{\alpha'^2} + \frac{2}{\alpha'} (N + \tilde{N} - 2)$.

1.2

Write the more explicit form of partition function Z^{25}

$$\begin{aligned} Z^{25} &= |\eta(q)|^{-2} \sum_{n,w=-\infty}^{+\infty} q^{\frac{\alpha' p_L^2}{4}} \bar{q}^{\frac{\alpha' p_R^2}{4}} \\ &= |\eta(q)|^{-2} \sum_{n,w=-\infty}^{+\infty} \exp 2\pi i(\tau_1 + i\tau_2) \times \frac{\alpha'}{4} \left(\frac{n}{R} + \frac{wR}{\alpha'} \right)^2 \times \end{aligned} \quad (1.13)$$

$$\times \exp -2\pi i(\tau_1 - i\tau_2) \times \frac{\alpha'}{4} \left(\frac{n}{R} - \frac{wR}{\alpha'} \right)^2 \quad (1.14)$$

Calculate the factor in exponential

$$\begin{aligned} &2\pi i(\tau_1 + i\tau_2) \times \frac{\alpha'}{4} \left(\frac{n}{R} + \frac{wR}{\alpha'} \right)^2 - 2\pi i(\tau_1 - i\tau_2) \times \frac{\alpha'}{4} \left(\frac{n}{R} - \frac{wR}{\alpha'} \right)^2 \\ &= 2\pi i\tau_1 \times \frac{\alpha'}{4} \times \frac{4nw}{\alpha'} - 2\pi\tau_2 \times \frac{\alpha'}{4} \times 2 \left(\frac{n^2}{R^2} + \frac{w^2 R^2}{\alpha'^2} \right) \\ &= 2\pi i\tau_1 nw - \pi\tau_2 \left(\frac{\alpha' n^2}{R^2} + \frac{w^2 R^2}{\alpha'} \right) \end{aligned} \quad (1.15)$$

The partition function now is

$$Z^{25} = |\eta(q)|^{-2} \sum_{n,w=-\infty}^{+\infty} \exp 2\pi i\tau_1 nw - \pi\tau_2 \left(\frac{\alpha' n^2}{R^2} + \frac{w^2 R^2}{\alpha'} \right) \quad (1.16)$$

Using the Poisson resummation formula.

$$\sum_{n=-\infty}^{\infty} \exp(-\pi a n^2 + 2\pi i b n) = a^{-1/2} \sum_{m=-\infty}^{\infty} \exp\left[-\frac{\pi(m-b)^2}{a}\right] \quad (1.17)$$

By replacement $a \rightarrow \frac{\tau_2 \alpha'}{R^2}$ and $b \rightarrow \tau_1 w$ the partition formula is

$$\begin{aligned} Z^{25} &= |\eta(q)|^{-2} \left(\frac{\tau_2 \alpha'}{R^2} \right)^{-1/2} \sum_{w=-\infty}^{+\infty} \exp\left(-\pi\tau_2 \frac{w^2 R^2}{\alpha'}\right) \sum_{m=-\infty}^{\infty} \exp\left[-\frac{\pi R^2 (m - \tau_1 w)^2}{\tau_2 \alpha'}\right] \\ &= |\eta(q)|^{-2} \left(\frac{\tau_2 \alpha'}{R^2} \right)^{-1/2} \sum_{w,m=-\infty}^{+\infty} \exp\left[-\frac{\pi R^2}{\tau_2 \alpha'} (\tau_2^2 w^2 + m^2 - 2m\tau_1 w + \tau_1^2 w^2)\right] \\ &= |\eta(q)|^{-2} \left(\frac{\tau_2 \alpha'}{R^2} \right)^{-1/2} \sum_{w,m=-\infty}^{+\infty} \exp\left[-\frac{\pi R^2}{\tau_2 \alpha'} |m - w\tau|^2\right] \end{aligned} \quad (1.18)$$

Now illustrate the modular invariance of the partition function. Under the transformation $\tau \rightarrow \tau + 1$, $\tau_2 \rightarrow \tau_2$, $\eta(\tau) \rightarrow e^{i\pi/12} \eta(\tau)$. Thus the partition function

changes

$$\begin{aligned}
Z^{25} &= |\eta(q)|^{-2} \left(\frac{\tau_2 \alpha'}{R^2} \right)^{-1/2} \sum_{w, m=-\infty}^{+\infty} \exp \left[-\frac{\pi R^2}{\tau_2 \alpha'} |m - w\tau|^2 \right] \\
&\rightarrow |\eta(q)|^{-2} \left(\frac{\tau_2 \alpha'}{R^2} \right)^{-1/2} \sum_{w, m=-\infty}^{+\infty} \exp \left[-\frac{\pi R^2}{\tau_2 \alpha'} |m - w(\tau + 1)|^2 \right] \quad (1.19)
\end{aligned}$$

is invariant if we replace the sum index m by $m + w$.

Under the transformation $\tau \rightarrow -1/\tau$, we have $\tau_2 \rightarrow \tau_2/|\tau|^2$, $\eta(\tau) \rightarrow \sqrt{-i\tau}\eta(\tau)$.

$$\begin{aligned}
Z^{25} &= |\eta(q)|^{-2} \left(\frac{\tau_2 \alpha'}{R^2} \right)^{-1/2} \sum_{w, m=-\infty}^{+\infty} \exp \left[-\frac{\pi R^2}{\tau_2 \alpha'} |m - w\tau|^2 \right] \\
&\rightarrow |\eta(q)|^{-2} \sqrt{\tau} \left(\frac{\tau_2 \alpha'}{R^2} \right)^{-1/2} \sqrt{\tau}^{-1} \sum_{w, m=-\infty}^{+\infty} \exp \left[-\frac{\pi R^2}{\tau_2 \alpha'} |\tau|^2 |m - w(-1/\tau)|^2 \right] \\
&= |\eta(q)|^{-2} \left(\frac{\tau_2 \alpha'}{R^2} \right)^{-1/2} \sum_{w, m=-\infty}^{+\infty} \exp \left[-\frac{\pi R^2}{\tau_2 \alpha'} |m\tau + w|^2 \right] \quad (1.20)
\end{aligned}$$

is invariant if we replace the sum index $m \rightarrow -w$ and $w \rightarrow m$.

1.3

In the case of self-dual $R = \sqrt{\alpha'}$. The partition function Z^{25} now is

$$\begin{aligned}
Z^{25} &= |\eta(q)|^{-2} \sum_{n, w=-\infty}^{+\infty} q^{\frac{\alpha' p_L^2}{4}} \bar{q}^{\frac{\alpha' p_R^2}{4}} \\
&= |\eta(q)|^{-2} \sum_{n, w=-\infty}^{+\infty} q^{\frac{(n+w)^2}{4}} \bar{q}^{\frac{(n-w)^2}{4}} \quad (1.21)
\end{aligned}$$

Do the replacement $n \rightarrow n - w$

$$\begin{aligned}
Z^{25} &= |\eta(q)|^{-2} \sum_{n, w=-\infty}^{+\infty} q^{\frac{n^2}{4}} \bar{q}^{\frac{(n-2w)^2}{4}} \\
&= |\eta(q)|^{-2} \sum_{w=-\infty}^{+\infty} \left(\sum_{2k+1, k \in \mathbb{Z}} q^{\frac{(2k+1)^2}{4}} \bar{q}^{\frac{(2k+1-2w)^2}{4}} + \sum_{2k, k \in \mathbb{Z}} q^{\frac{(2k)^2}{4}} \bar{q}^{\frac{(2k-2w)^2}{4}} \right) \\
&= |\eta(q)|^{-2} \sum_{w, k=-\infty}^{+\infty} q^{(k+1/2)^2} \bar{q}^{(k-w+1/2)^2} + q^{k^2} \bar{q}^{(k-w)^2} \quad (1.22)
\end{aligned}$$

With the replacement $w \rightarrow -w + k$, we have

$$\begin{aligned}
Z^{25} &= |\eta(q)|^{-2} \sum_{w,k=-\infty}^{+\infty} q^{(k+1/2)^2} \bar{q}^{(w+1/2)^2} + q^{k^2} \bar{q}^{w^2} \\
&= \left| \eta^{-1} \sum_{n \in \mathbb{Z}} q^{n^2} \right|^2 + \left| \eta^{-1} \sum_{n \in \mathbb{Z}} q^{n^2+1/2} \right|^2 \\
&= |\chi_1(q)|^2 + |\chi_2(q)|^2
\end{aligned} \tag{1.23}$$

The χ_i are the characters of the $SU(2)$ affine Lie algebra with level $k = 1$. Now the whole partition function is

$$Z^{1,24} Z^{25} = \text{const} \times |\eta(q)|^{-48} \sum_{w,k=-\infty}^{+\infty} q^{(k+1/2)^2} \bar{q}^{(w+1/2)^2} + q^{k^2} \bar{q}^{w^2} \tag{1.24}$$

According to lecture note 8, first factor $|\eta(q)|^{-48} \simeq |q^{-1} + 24 + O(q)|^2$. Its easy to see that the terms with $k = w = 0$ in the second factor contribute to usual 24 bosonic massless states. However $|q|^2$, q , \bar{q} terms in the the second factor gives contributions to additional massless states, which corresponds to eight cases $k, w = \pm 1$, $k = 0, w = \pm 1$ and $k = \pm 1, w = 0$.

We now briefly conclude these cases. We denote w, n in original partition function as w_o, n_o

$$\begin{aligned}
k = w = \pm 1 & \quad n_o = \pm 2 & \quad w_o = 0 & \quad N = \tilde{N} = 0 \\
k = -w = \pm 1 & \quad n_o = 0 & \quad w_o = \pm 2 & \quad N = \tilde{N} = 0 \\
k = \pm 1 & \quad w = 0 & \quad n_o = w_o = \pm 1 & \quad N = 0 \quad \tilde{N} = 1 \\
k = 0 & \quad w = \pm 1 & \quad n_o = -w_o = \pm 1 & \quad N = 1 \quad \tilde{N} = 0
\end{aligned}$$

The last four states are physical additional massless states with nonzero state number.

1.4

The current in the bosonic string theory is defined by

$$\begin{aligned}
j^\pm(z) &= j^1(z) \pm i j^2(z) :- e^{\pm 2iX^{25}(z)/\sqrt{\alpha'}} \\
j^3(z) &:- i \partial X^{25}(z)/\sqrt{\alpha'}
\end{aligned} \tag{1.25}$$

so we can write $j^1(z)$ and $j^2(z)$

$$j^1(z) = \frac{1}{2}(j^+(z) + j^-(z)) = \frac{1}{2}(e^{2iX^{25}(z)/\sqrt{\alpha'}} + e^{-2iX^{25}(z)/\sqrt{\alpha'}}) \tag{1.26}$$

$$j^2(z) = \frac{1}{2i}(j^+(z) - j^-(z)) = \frac{1}{2i}(e^{2iX^{25}(z)/\sqrt{\alpha'}} - e^{-2iX^{25}(z)/\sqrt{\alpha'}}) \tag{1.27}$$

Useful formula which have proved in previous notes or exercises:

$$X^{25}(z)X^{25}(0) \sim -\frac{\alpha'}{2} \ln z \quad (1.28)$$

$$: e^{ik_1 X^{25}(z)} :: e^{ik_2 X^{25}(0)} : = z^{\frac{\alpha'}{2} k_1 k_2} : e^{ik_1 X^{25}(z)} e^{ik_2 X^{25}(0)} : \quad (1.29)$$

$$: \partial X^{25}(z) :: e^{ik X^{25}(0)} : \sim \partial(-\frac{\alpha'}{2} \ln z) ik : e^{ik X^{25}(0)} : \quad (1.30)$$

Calculate OPE $j^3 j^3$

$$j^3(z)j^3(0) = -\frac{1}{\alpha'} \partial X^{25}(z) \partial X^{25}(0) \sim \frac{1}{\alpha'} \partial^2(-\frac{\alpha'}{2} \ln z) = \frac{1}{2z^2} \quad (1.31)$$

OPE $j^1 j^1$

$$\begin{aligned} j^1(z)j^1(0) &= \frac{1}{4} : (e^{2iX^{25}(z)/\sqrt{\alpha'}} + e^{-2iX^{25}(z)/\sqrt{\alpha'}}) :: (e^{2iX^{25}(0)/\sqrt{\alpha'}} + e^{-2iX^{25}(0)/\sqrt{\alpha'}}) : \\ &= \frac{1}{4} \left(z^2 : e^{2iX^{25}(z)/\sqrt{\alpha'}} e^{2iX^{25}(0)/\sqrt{\alpha'}} : + z^{-2} : e^{2iX^{25}(z)/\sqrt{\alpha'}} e^{-2iX^{25}(0)/\sqrt{\alpha'}} : + \right. \\ &\quad \left. + z^{-2} : e^{-2iX^{25}(z)/\sqrt{\alpha'}} e^{2iX^{25}(0)/\sqrt{\alpha'}} : + z^2 : e^{-2iX^{25}(z)/\sqrt{\alpha'}} e^{-2iX^{25}(0)/\sqrt{\alpha'}} : \right) \\ &= \frac{1}{4} \left[z^{-2} \left(1 + \frac{2i}{\sqrt{\alpha'}} \partial X^{25}(0) z + O(z^2) \right) + z^{-2} \left(1 - \frac{2i}{\sqrt{\alpha'}} \partial X^{25}(0) z + O(z^2) \right) + O(z^2) \right] \\ &= \frac{1}{2z^2} + O(z^2) \\ &\sim \frac{1}{2z^2} \end{aligned} \quad (1.32)$$

Similar for OPE $j^2 j^2$

$$\begin{aligned} j^2(z)j^2(0) &= -\frac{1}{4} : (e^{2iX^{25}(z)/\sqrt{\alpha'}} - e^{-2iX^{25}(z)/\sqrt{\alpha'}}) :: (e^{2iX^{25}(0)/\sqrt{\alpha'}} - e^{-2iX^{25}(0)/\sqrt{\alpha'}}) : \\ &= -\frac{1}{4} \left(z^2 : e^{2iX^{25}(z)/\sqrt{\alpha'}} e^{2iX^{25}(0)/\sqrt{\alpha'}} : - z^{-2} : e^{2iX^{25}(z)/\sqrt{\alpha'}} e^{-2iX^{25}(0)/\sqrt{\alpha'}} : + \right. \\ &\quad \left. - z^{-2} : e^{-2iX^{25}(z)/\sqrt{\alpha'}} e^{2iX^{25}(0)/\sqrt{\alpha'}} : + z^2 : e^{-2iX^{25}(z)/\sqrt{\alpha'}} e^{-2iX^{25}(0)/\sqrt{\alpha'}} : \right) \\ &= \frac{1}{4} \left[z^{-2} \left(1 + \frac{2i}{\sqrt{\alpha'}} \partial X^{25}(0) z + O(z^2) \right) + z^{-2} \left(1 - \frac{2i}{\sqrt{\alpha'}} \partial X^{25}(0) z + O(z^2) \right) + O(z^2) \right] \\ &= \frac{1}{2z^2} + O(z^2) \\ &\sim \frac{1}{2z^2} \end{aligned} \quad (1.33)$$

Calculate OPE $j^3 j^1$

$$\begin{aligned}
j^3(z)j^1(0) &= \frac{i}{2\sqrt{\alpha'}} \partial X^{25}(z) : (e^{2iX^{25}(0)/\sqrt{\alpha'}} + e^{-2iX^{25}(0)/\sqrt{\alpha'}}) : \\
&\sim \frac{i}{2\sqrt{\alpha'}} \left(-\frac{\alpha'}{2} \times \frac{2i}{\sqrt{\alpha'}} z^{-1} : e^{2iX^{25}(0)/\sqrt{\alpha'}} : -\frac{\alpha'}{2} \times \frac{-2i}{\sqrt{\alpha'}} z^{-1} : e^{-2iX^{25}(0)/\sqrt{\alpha'}} : \right) \\
&= \frac{i}{z} \frac{1}{2i} \left(: e^{2iX^{25}(0)/\sqrt{\alpha'}} : - : e^{-2iX^{25}(0)/\sqrt{\alpha'}} : \right) \\
&= \frac{i}{z} j^2(0)
\end{aligned} \tag{1.34}$$

When calculate OPE $j^1 j^3$, the ∂ in j^3 act on "0" offer an extra minus sign, so we have

$$j^1(z)j^3(0) \sim -\frac{i}{z} j^2(0) \tag{1.35}$$

Similar calculation for OPE $j^3 j^2$

$$\begin{aligned}
j^3(z)j^2(0) &= \frac{1}{2\sqrt{\alpha'}} \partial X^{25}(z) : (e^{2iX^{25}(0)/\sqrt{\alpha'}} - e^{-2iX^{25}(0)/\sqrt{\alpha'}}) : \\
&\sim \frac{1}{2\sqrt{\alpha'}} \left(-\frac{\alpha'}{2} \times \frac{2i}{\sqrt{\alpha'}} z^{-1} : e^{2iX^{25}(0)/\sqrt{\alpha'}} : + \frac{\alpha'}{2} \times \frac{-2i}{\sqrt{\alpha'}} z^{-1} : e^{-2iX^{25}(0)/\sqrt{\alpha'}} : \right) \\
&= -\frac{i}{z} \frac{1}{2} \left(: e^{2iX^{25}(0)/\sqrt{\alpha'}} : + : e^{-2iX^{25}(0)/\sqrt{\alpha'}} : \right) \\
&= -\frac{i}{z} j^1(0)
\end{aligned} \tag{1.36}$$

$$j^2(z)j^3(0) = \frac{i}{z} j^1(0) \tag{1.37}$$

Finally, we goes to OPE $j^1 j^2$

$$\begin{aligned}
j^1(z)j^2(0) &= \frac{1}{4i} : (e^{2iX^{25}(z)/\sqrt{\alpha'}} + e^{-2iX^{25}(z)/\sqrt{\alpha'}}) :: (e^{2iX^{25}(0)/\sqrt{\alpha'}} - e^{-2iX^{25}(0)/\sqrt{\alpha'}}) : \\
&= \frac{1}{4i} \left(z^2 : e^{2iX^{25}(z)/\sqrt{\alpha'}} e^{2iX^{25}(0)/\sqrt{\alpha'}} : - z^{-2} : e^{2iX^{25}(z)/\sqrt{\alpha'}} e^{-2iX^{25}(0)/\sqrt{\alpha'}} : + \right. \\
&\quad \left. + z^{-2} : e^{-2iX^{25}(z)/\sqrt{\alpha'}} e^{2iX^{25}(0)/\sqrt{\alpha'}} : - z^2 : e^{-2iX^{25}(z)/\sqrt{\alpha'}} e^{-2iX^{25}(0)/\sqrt{\alpha'}} : \right) \\
&= \frac{1}{4i} \left[-z^{-2} \left(1 + \frac{2i}{\sqrt{\alpha'}} \partial X^{25}(0) z + O(z^2) \right) + z^{-2} \left(1 - \frac{2i}{\sqrt{\alpha'}} \partial X^{25}(0) z + O(z^2) \right) + O(z^2) \right] \\
&\sim \frac{i}{z} \frac{i}{\sqrt{\alpha'}} \partial X^{25}(0) = \frac{i}{z} j^3(0)
\end{aligned} \tag{1.38}$$

Follow the similar pattern we have

$$j^2(z)j^1(0) \sim -\frac{i}{z} \frac{i}{\sqrt{\alpha'}} \partial X^{25}(0) = -\frac{i}{z} j^3(0) \tag{1.39}$$

Thus the OPE can be concluded

$$j^a(z)j^b(0) \sim \frac{\delta^{ab}}{2z^2} + \frac{i\epsilon^{abc}j^c(0)}{z} \quad (1.40)$$

The oscillator modes of the currents

$$j^a(z) = \sum_{m \in \mathbb{Z}} \frac{j_m^a}{z^{m+1}} \quad (1.41)$$

So we have

$$j_m^a = \oint_c \frac{dz}{2\pi i} z^m j^a(z) \quad (1.42)$$

The commutator $[j_m^a, j_n^b]$ is

$$\begin{aligned} [j_m^a, j_n^b] &= \left(\oint_{c_1} \oint_{c_2} - \oint_{c_2} \oint_{c_3} \right) \frac{dz}{2\pi i} \frac{dw}{2\pi i} z^m w^n j^a(z) j^b(w) \\ &= \oint_{c_2} \frac{dw}{2\pi i} \oint_{c_W} \frac{dz}{2\pi i} z^m w^n \left[\frac{\delta^{ab}}{2(z-w)^2} + \frac{i\epsilon^{abc}j^c(w)}{z-w} \right] \\ &= \oint_{c_2} \frac{dw}{2\pi i} \left[\frac{1}{2} m \omega^{n+m-1} \delta^{ab} + i\epsilon^{abc} j^c(\omega) \omega^{m+n} \right] \\ &= \delta_{n+m,0} \frac{1}{2} m \delta^{ab} + i\epsilon^{abc} j_{m+n}^c \end{aligned} \quad (1.43)$$

2 RR field strengths and T-duality in Type II

The Clifford algebra of $SO(1,9)$ gamma matrices defined as

$$\{\Gamma^\mu, \Gamma^\nu\} = 2\eta^{\mu\nu} \quad \mu, \nu = 0, 1 \dots 9 \quad (2.1)$$

The chirality matrix is $\Gamma^{11} = \Gamma^0 \Gamma^1 \dots \Gamma^9$, calculate $\Gamma^{11} \Gamma^{11}$:

$$\Gamma^{11} \Gamma^{11} = \Gamma^0 \Gamma^1 \dots \Gamma^9 \Gamma^0 \Gamma^1 \dots \Gamma^9 = (-1)^{9+8+\dots+1} (\Gamma^0)^2 (\Gamma^1)^2 \dots (\Gamma^9)^2 = (-1)^{46} = 1 \quad (2.2)$$

The anticommutator of Γ^{11} and Γ^μ vanishes

$$\{\Gamma^{11}, \Gamma^\mu\} = \Gamma^{11} \Gamma^\mu + \Gamma^\mu \Gamma^{11} = \Gamma^{11} \Gamma^\mu + (-1)^9 \Gamma^{11} \Gamma^\mu = 0 \quad (2.3)$$

Chiral spinors are now defined by $\Gamma^{11} \psi_\pm = \pm \psi_\pm$, then we have

$$\bar{\psi}_\pm \Gamma^{11} = \psi_\pm^\dagger \Gamma^0 \Gamma^{11} = (\Gamma^{11\dagger} \Gamma^{0\dagger} \psi_\pm)^\dagger \quad (2.4)$$

Notice that

$$\Gamma^{11\dagger} = \Gamma^{9\dagger} \dots \Gamma^{0\dagger} = \Gamma^0 \Gamma^9 \Gamma^8 \dots \Gamma^0 (\Gamma^0)^{-1} = (-1)^{45} \Gamma^0 \Gamma^0 \Gamma^1 \dots \Gamma^9 (\Gamma^0)^{-1} = -\Gamma^0 \Gamma^{11} (\Gamma^0)^{-1} \quad (2.5)$$

So, we have

$$\bar{\psi}_{\pm}\Gamma^{11} = (\Gamma^0\Gamma^{11}\Gamma^0(\Gamma^0)^{-1}\psi_{\pm})^{\dagger} = \pm(\Gamma^0\psi_{\pm})^{\dagger} = \pm\psi_{\pm}^{\dagger}(-\Gamma^0) = \mp\bar{\psi}_{\pm} \quad (2.6)$$

The R R field strengths $G_{\mu_1\cdots\mu_{p+1}}$ as bilinears

$$\text{II A : } \quad \bar{\psi}_{-}^L\Gamma^{\mu_1\cdots\mu_{p+1}}\psi_{+}^R \quad \text{II B : } \quad \bar{\psi}_{+}^L\Gamma^{\mu_1\cdots\mu_{p+1}}\psi_{+}^R \quad (2.7)$$

Since the spacetime indexes are antisymmetric $p+1 \leq 10$. Consider Type II A

$$\bar{\psi}_{-}^L\Gamma^{\mu_1\cdots\mu_{p+1}}\psi_{+}^R = \bar{\psi}_{-}^L\Gamma^{11}\Gamma^{\mu_1\cdots\mu_{p+1}}\Gamma^{11}\psi_{+}^R = \bar{\psi}_{-}^L(\Gamma^{11})^2(-1)^{p+1}\Gamma^{\mu_1\cdots\mu_{p+1}}\psi_{+}^R = (-1)^{p+1}\bar{\psi}_{-}^L\Gamma^{\mu_1\cdots\mu_{p+1}}\psi_{+}^R \quad (2.8)$$

So, for type II A, the spinor bilinears will vanish unless p is odd. p can be 1, 3, 5, 7, 9. Similar for Type II B

$$\bar{\psi}_{+}^L\Gamma^{\mu_1\cdots\mu_{p+1}}\psi_{+}^R = -\bar{\psi}_{+}^L\Gamma^{11}\Gamma^{\mu_1\cdots\mu_{p+1}}\Gamma^{11}\psi_{+}^R = (-1)^{p+2}\bar{\psi}_{+}^L\Gamma^{\mu_1\cdots\mu_{p+1}}\psi_{+}^R \quad (2.9)$$

For type II B, the spinor bilinears will vanish unless p is even. So p can be 0, 2, 4, 6, 8. Since $\beta_9 = \Gamma^9\Gamma^{11}$, we have

$$\{\beta_9, \Gamma^9\} = \{\Gamma^9\Gamma^{11}, \Gamma^9\} = \Gamma^9\{\Gamma^{11}, \Gamma^9\} - [\Gamma^9, \Gamma^9]\Gamma^{11} = 0 \quad (2.10)$$

For $\mu \neq 9$

$$[\beta_9, \Gamma^{\mu}] = [\Gamma^9\Gamma^{11}, \Gamma^{\mu}] = \Gamma^9\{\Gamma^{11}, \Gamma^{\mu}\} - \{\Gamma^9, \Gamma^{\mu}\}\Gamma^{11} = 0 \quad (2.11)$$

Under T-duality transformation $\psi^L \rightarrow \psi^L$, $\psi^R \rightarrow \beta_9\psi^R$

$$\bar{\psi}_{-}^L\Gamma^{\mu_1\cdots\mu_{p+1}}\psi_{+}^R \rightarrow \bar{\psi}_{-}^L\Gamma^{\mu_1\cdots\mu_{p+1}}\beta_9\psi_{+}^R \quad (2.12)$$

Follow the same step, we see that

$$\bar{\psi}_{-}^L\Gamma^{\mu_1\cdots\mu_{p+1}}\beta_9\psi_{+}^R = \bar{\psi}_{-}^L\Gamma^{11}\Gamma^{\mu_1\cdots\mu_{p+1}}\beta_9\Gamma^{11}\psi_{+}^R = (-1)^{p+2}\bar{\psi}_{-}^L\Gamma^{\mu_1\cdots\mu_{p+1}}\beta_9\psi_{+}^R \quad (2.13)$$

The transformed spinor bilinear vanishes unless p is even which is the case of type II B. And we find $\bar{\psi}_{-}^L\Gamma^{\mu_1\cdots\mu_{p+1}}\beta_9\psi_{+}^R \sim \bar{\psi}_{-}^L\beta_9\Gamma^{\mu_1\cdots\mu_{p+1}}\psi_{+}^R$ up to a sign factor. And

$$\bar{\psi}_{-}^L\beta_9\Gamma^{11} = -\bar{\psi}_{-}^L\Gamma^{11}\beta_9 = +\bar{\psi}_{-}^L\beta_9 \quad (2.14)$$

So $\bar{\psi}_{-}^L\beta_9 \sim \bar{\psi}_{-}^L$. Thus T duality transform RR field strengths in II A to II B, and the same reason vice versa.

$$\bar{\psi}_{+}^L\Gamma^{\mu_1\cdots\mu_{p+1}}\psi_{+}^R \rightarrow \bar{\psi}_{+}^L\Gamma^{\mu_1\cdots\mu_{p+1}}\beta_9\psi_{+}^R \quad (2.15)$$

$$\bar{\psi}_{+}^L\Gamma^{\mu_1\cdots\mu_{p+1}}\beta_9\psi_{+}^R = \bar{\psi}_{+}^L\Gamma^{11}\Gamma^{\mu_1\cdots\mu_{p+1}}\beta_9\Gamma^{11}\psi_{+}^R = (-1)^{p+2}\bar{\psi}_{+}^L\Gamma^{\mu_1\cdots\mu_{p+1}}\beta_9\psi_{+}^R \quad (2.16)$$

The transformed spinor bilinear vanishes unless p is odd which is the case of type II A. And we find $\bar{\psi}_{+}^L\Gamma^{\mu_1\cdots\mu_{p+1}}\beta_9\psi_{+}^R \sim \bar{\psi}_{+}^L\beta_9\Gamma^{\mu_1\cdots\mu_{p+1}}\psi_{+}^R$ up to a sign factor. And

$$\bar{\psi}_{+}^L\beta_9\Gamma^{11} = -\bar{\psi}_{+}^L\Gamma^{11}\beta_9 = -\bar{\psi}_{+}^L\beta_9 \quad (2.17)$$

So $\bar{\psi}_{+}^L\beta_9 \sim \bar{\psi}_{+}^L$.

3 D-branes in Type II and T- duality

3.1

Since T-duality exchange NN to DD and ND to DN in corresponding spacetime direction, the number ($\# \text{ NN} + \# \text{ DD}$) and ($\# \text{ ND} + \# \text{ DN}$) are invariant.

3.2

Without loss of generality, we place all the spacetime dimension as small as possible. For II B theory p must be odd .Above tables list all the possible configuration, and all these configurations are dual to the D1-D5 configuration.

	0	1	2	3	4	5	6	7	8	9
D3	×	×	×	×						
D1	×				×					

Table 1: transform to D1-D5 by T_4, T_5

	0	1	2	3	4	5	6	7	8	9
D3	×	×	×	×						
D3	×	×			×	×				

Table 2: transform to D1-D5 by T_2, T_3

	0	1	2	3	4	5	6	7	8	9
D3	×	×	×	×						
D5	×	×	×		×	×	×			

Table 3: transform to D1-D5 by T_1, T_3

	0	1	2	3	4	5	6	7	8	9
D3	×	×	×	×						
D5	×	×	×	×	×	×	×	×		

Table 4: transform to D1-D5 by T_1, T_2